coq: ZF: refactor

coq/ZF/Meta/Test/Axiom/Choice.v
@@ -2,17 +2,34 @@ Require Import Coq.Lists.List.
 Require Import Coq.Strings.String.
 
 Require Import ZF.Meta.Ctx.
-Require Import ZF.Meta.Sigs.
+Require Import ZF.Meta.Decl.
+Require Import ZF.Meta.Env.
 Require Import ZF.Meta.Term.
 Require Import ZF.Meta.HasTy.
+Require Import ZF.Meta.HasTyIn.
 Require Import ZF.Meta.Ty.
 
 Import ListNotations.
 
-Definition sigs : Sigs := fun name =>
-  if String.eqb name "FunctionOn" then Some ([TySet; TySet], TyProp) else
-  if String.eqb name "empty"      then Some ([]              , TySet ) else
-  if String.eqb name "eval"       then Some ([TySet; TySet], TySet ) else
+Definition FunctionOn : Decl :=
+  {| para := [TySet; TySet];
+     res  := TyProp;
+     body := None |}.
+
+Definition empty : Decl :=
+  {| para := [];
+     res  := TySet;
+     body := None |}.
+
+Definition eval : Decl :=
+  {| para := [TySet; TySet];
+     res  := TySet;
+     body := None |}.
+
+Definition env : Env := fun name =>
+  if String.eqb name "FunctionOn" then Some FunctionOn else
+  if String.eqb name "empty"      then Some empty else
+  if String.eqb name "eval"       then Some eval else
   None.
 
 (* forall a,                                                                    *)
@@ -29,9 +46,10 @@ Definition Choice : Term :=
               (NotEq (Var 0) (Ident "empty" []))
               (Elem (Ident "eval" [Var 1; Var 0]) (Var 0))))))).
 
-(* The choice example is a proposition in the local test signature.             *)
-Proposition HasTy : HasTy sigs Ctx.empty Choice TyProp.
+(* The choice example is a proposition in the local test environment.           *)
+Proposition HasTy : HasTyIn env Ctx.empty Choice TyProp.
 Proof.
+  (* Proof by Hermes + gpt 5.5                                                  *)
   apply HasTyAll, HasTyEx, HasTyAnd.
   - apply HasTyIdent with (argTys := [TySet; TySet]). 1: reflexivity.
     apply HasTysCons.
