coq/ZF/Meta/HasTyIn.v
@@ -1,0 +1,9 @@
+Require Import ZF.Meta.Ctx.
+Require Import ZF.Meta.Env.
+Require Import ZF.Meta.HasTy.
+Require Import ZF.Meta.Term.
+Require Import ZF.Meta.Ty.
+
+(* A term is well typed in an environment through its signatures view.          *)
+Definition HasTyIn (e:Env) (G:Ctx) (t:Term) (ty:Ty) : Prop :=
+  HasTy (Env.toSigs e) G t ty.
